generational/spec/GC.Gen.CheneyPreservation.Injectivity.fst
@@ -1,0 +1,735 @@
+/// ---------------------------------------------------------------------------
+/// GC.Gen.CheneyPreservation.Injectivity -- forwarding injectivity
+/// ---------------------------------------------------------------------------
+
+module GC.Gen.CheneyPreservation.Injectivity
+
+open FStar.Seq
+module U64 = FStar.UInt64
+
+open GC.Spec.Base
+open GC.Spec.Heap
+open GC.Spec.Object
+open GC.Spec.Fields
+open GC.Gen.Base
+open GC.Gen.MinorHeap
+open GC.Gen.Promote
+open GC.Gen.PromoteUpdate
+open GC.Gen.Cheney
+open GC.Gen.WriteBodyLemmas
+open GC.Lib.Header
+
+module Allocator = GC.Spec.Allocator
+module AllocLemmas = GC.Spec.Allocator.Lemmas
+module AllocProps = GC.Gen.AllocProps
+open GC.Gen.CheneyPreservation.Forwarding
+
+/// ---------------------------------------------------------------------------
+/// Injectivity
+/// ---------------------------------------------------------------------------
+
+let inj_inv (cs: cheney_state) : prop =
+  fwd_normal_injective cs.cs_fwd cs.cs_major /\
+  fwd_targets_not_blue cs.cs_fwd cs.cs_major
+
+#push-options "--z3rlimit 40 --fuel 0 --ifuel 0"
+private let chain_avoids_from_blue
+  (major: heap) (fp: U64.t) (obj: obj_addr)
+  : Lemma
+    (requires chain_objects_blue major fp /\
+              Seq.mem obj (objects zero_addr major) /\
+              is_blue obj major = false)
+    (ensures AllocLemmas.chain_avoids major fp obj (heap_size / U64.v mword) = true)
+  = reveal_opaque (`%chain_objects_blue) chain_objects_blue
+#pop-options
+
+#push-options "--z3rlimit 80 --fuel 1 --ifuel 0 --split_queries always"
+private let cheney_forward_normal_preserves_wfh_part4_local
+  (minor: minor_state) (cs: cheney_state) (addr: U64.t)
+  : Lemma (requires well_formed_heap_part4 cs.cs_major /\
+                    well_formed_heap_part1 cs.cs_major /\
+                    AllocLemmas.fl_valid cs.cs_major cs.cs_fp (heap_size / U64.v mword) /\
+                    AllocLemmas.fl_chain_terminates cs.cs_major cs.cs_fp (heap_size / U64.v mword) /\
+                    minor_wf minor)
+          (ensures well_formed_heap_part4 (cheney_forward_normal minor cs addr).cs_major)
+  =
+  if not (Seq.mem addr (minor_objects minor)) || cs.cs_fwd addr <> 0UL
+  then begin
+    cheney_forward_normal_noop minor cs addr;
+    assert (cheney_forward_normal minor cs addr == cs)
+  end
+  else
+    let wz = minor_wosize minor addr in
+    if wz = 0 then begin
+      cheney_forward_normal_noop_wz0 minor cs addr;
+      assert (cheney_forward_normal minor cs addr == cs)
+    end
+    else begin
+      assert (Seq.mem addr (minor_objects minor));
+      assert (cs.cs_fwd addr = 0UL);
+      assert (wz > 0);
+      minor_objects_not_infix minor addr;
+      GC.Spec.Object.infix_tag_val ();
+      assert (minor_tag minor addr <> 249);
+      assert (U64.v GC.Spec.Object.infix_tag == 249);
+      assert (minor_tag minor addr <> U64.v GC.Spec.Object.infix_tag);
+      promote_object_preserves_wfh_part4 minor cs.cs_major addr cs.cs_fp wz;
+      let res = promote_object minor cs.cs_major addr cs.cs_fp wz in
+      if res.new_addr = 0UL then begin
+        cheney_forward_normal_noop_oom minor cs addr;
+        assert (cheney_forward_normal minor cs addr == cs)
+      end else begin
+        cheney_forward_normal_success minor cs addr;
+        assert ((cheney_forward_normal minor cs addr).cs_major == res.major_out);
+        assert (well_formed_heap_part4 res.major_out)
+      end
+    end
+#pop-options
+
+#push-options "--z3rlimit 80 --fuel 1 --ifuel 0 --split_queries always"
+private let cheney_forward_one_preserves_wfh_part4_local
+  (minor: minor_state) (cs: cheney_state) (addr: U64.t)
+  : Lemma (requires well_formed_heap_part4 cs.cs_major /\
+                    well_formed_heap_part1 cs.cs_major /\
+                    AllocLemmas.fl_valid cs.cs_major cs.cs_fp (heap_size / U64.v mword) /\
+                    AllocLemmas.fl_chain_terminates cs.cs_major cs.cs_fp (heap_size / U64.v mword) /\
+                    minor_wf minor /\
+                    minor_infix_wf minor)
+          (ensures well_formed_heap_part4 (cheney_forward_one minor cs addr).cs_major)
+  =
+  if cs.cs_fwd addr <> 0UL then begin
+    cheney_forward_one_noop minor cs addr;
+    assert (cheney_forward_one minor cs addr == cs)
+  end
+  else if is_infix_in_minor minor addr then begin
+    reveal_opaque (`%minor_infix_wf) (minor_infix_wf minor);
+    let parent = infix_parent minor addr in
+    infix_parent_value minor addr;
+    assert (U64.v parent == U64.v addr - minor_wosize minor addr * 8);
+    assert (U64.v addr >= U64.v parent);
+    cheney_forward_one_infix minor cs addr;
+    cheney_forward_normal_preserves_wfh_part4_local minor cs parent;
+    cheney_forward_normal_preserves_wfh_part1 minor cs parent;
+    let cs' = cheney_forward_normal minor cs parent in
+    assert ((cheney_forward_one minor cs addr).cs_major == cs'.cs_major);
+    assert (well_formed_heap_part4 (cheney_forward_one minor cs addr).cs_major)
+  end
+  else begin
+    cheney_forward_one_normal minor cs addr;
+    cheney_forward_normal_preserves_wfh_part4_local minor cs addr;
+    assert (cheney_forward_one minor cs addr ==
+      cheney_forward_normal minor cs addr)
+  end
+#pop-options
+
+#push-options "--z3rlimit 40 --fuel 1 --ifuel 0"
+private let rec cheney_forward_fields_preserves_wfh_part4_local
+  (minor: minor_state) (cs: cheney_state) (parent: U64.t) (idx: nat) (wosize: nat)
+  : Lemma (requires well_formed_heap_part4 cs.cs_major /\
+                    well_formed_heap_part1 cs.cs_major /\
+                    AllocLemmas.fl_valid cs.cs_major cs.cs_fp (heap_size / U64.v mword) /\
+                    AllocLemmas.fl_chain_terminates cs.cs_major cs.cs_fp (heap_size / U64.v mword) /\
+                    minor_wf minor /\
+                    minor_infix_wf minor)
+          (ensures well_formed_heap_part4 (cheney_forward_fields minor cs parent idx wosize).cs_major)
+          (decreases (if idx < wosize then wosize - idx else 0))
+  =
+  if idx >= wosize then
+    cheney_forward_fields_base minor cs parent idx wosize
+  else begin
+    cheney_forward_fields_step minor cs parent idx wosize;
+    let field_val = to_minor_offset (minor_read_field minor parent idx) in
+    cheney_forward_one_preserves_wfh_part4_local minor cs field_val;
+    cheney_forward_one_preserves_wfh_part1 minor cs field_val;
+    let cs' = cheney_forward_one minor cs field_val in
+    cheney_forward_fields_preserves_wfh_part4_local minor cs' parent (idx + 1) wosize
+  end
+#pop-options
+
+#push-options "--z3rlimit 40 --fuel 1 --ifuel 0"
+private let rec cheney_forward_roots_preserves_wfh_part4_local
+  (minor: minor_state) (cs: cheney_state) (roots: seq U64.t) (idx: nat)
+  : Lemma (requires well_formed_heap_part4 cs.cs_major /\
+                    well_formed_heap_part1 cs.cs_major /\
+                    AllocLemmas.fl_valid cs.cs_major cs.cs_fp (heap_size / U64.v mword) /\
+                    AllocLemmas.fl_chain_terminates cs.cs_major cs.cs_fp (heap_size / U64.v mword) /\
+                    minor_wf minor /\
+                    minor_infix_wf minor)
+          (ensures well_formed_heap_part4 (cheney_forward_roots minor cs roots idx).cs_major)
+          (decreases (if idx < Seq.length roots then Seq.length roots - idx else 0))
+  =
+  if idx >= Seq.length roots then
+    cheney_forward_roots_base minor cs roots idx
+  else begin
+    cheney_forward_roots_step minor cs roots idx;
+    let r = Seq.index roots idx in
+    cheney_forward_one_preserves_wfh_part4_local minor cs r;
+    cheney_forward_one_preserves_wfh_part1 minor cs r;
+    let cs' = cheney_forward_one minor cs r in
+    cheney_forward_roots_preserves_wfh_part4_local minor cs' roots (idx + 1)
+  end
+#pop-options
+
+#push-options "--z3rlimit 50 --fuel 1 --ifuel 0 --split_queries always"
+private let rec cheney_scan_preserves_wfh_part4_local
+  (minor: minor_state) (cs: cheney_state) (scan: nat) (fuel: nat)
+  : Lemma (requires well_formed_heap_part4 cs.cs_major /\
+                    well_formed_heap_part1 cs.cs_major /\
+                    AllocLemmas.fl_valid cs.cs_major cs.cs_fp (heap_size / U64.v mword) /\
+                    AllocLemmas.fl_chain_terminates cs.cs_major cs.cs_fp (heap_size / U64.v mword) /\
+                    minor_wf minor /\
+                    minor_infix_wf minor)
+          (ensures well_formed_heap_part4 (cheney_scan minor cs scan fuel).cs_major)
+          (decreases fuel)
+  =
+  if fuel > 0 then begin
+    if scan >= Seq.length cs.cs_queue then
+      cheney_scan_base minor cs scan fuel
+    else begin
+      cheney_scan_step minor cs scan fuel;
+      let obj = Seq.index cs.cs_queue scan in
+      let wz = minor_wosize minor obj in
+      cheney_forward_fields_preserves_wfh_part4_local minor cs obj 0 wz;
+      cheney_forward_fields_preserves_wfh_part1 minor cs obj 0 wz;
+      let cs' = cheney_forward_fields minor cs obj 0 wz in
+      let fuel' : nat = fuel - 1 in
+      assert (fuel' < fuel);
+      cheney_scan_preserves_wfh_part4_local minor cs' (scan + 1) fuel'
+    end
+  end else
+    cheney_scan_base minor cs scan fuel
+#pop-options
+
+#push-options "--z3rlimit 120 --fuel 1 --ifuel 0 --split_queries always"
+private let promote_object_preserves_old_target_not_blue
+  (minor: minor_state) (major: heap) (obj: U64.t) (fp: U64.t) (wz: nat{wz > 0})
+  (target: obj_addr)
+  : Lemma
+    (requires well_formed_heap_part1 major /\
+              AllocLemmas.fl_valid major fp (heap_size / U64.v mword) /\
+              AllocLemmas.fl_chain_terminates major fp (heap_size / U64.v mword) /\
+              chain_objects_blue major fp /\
+              (promote_object minor major obj fp wz).new_addr <> 0UL /\
+              Seq.mem target (objects zero_addr major) /\
+              is_blue target major = false)
+    (ensures
+      (let res = promote_object minor major obj fp wz in
+       Seq.mem target (objects zero_addr res.major_out) /\
+       is_blue target res.major_out = false))
+  =
+  let res = promote_object minor major obj fp wz in
+  promote_object_success minor major obj fp wz;
+  promote_object_preserves_objects_part1 minor major obj fp wz;
+  chain_avoids_from_blue major fp target;
+  AllocProps.alloc_spec_obj_ne_excl major fp wz target;
+  assert (res.new_addr <> target);
+  promote_object_frame_old_header_derived minor major obj fp wz target;
+  color_of_header_eq target major res.major_out;
+  is_blue_iff target major;
+  is_blue_iff target res.major_out
+#pop-options
+
+#push-options "--z3rlimit 300 --fuel 1 --ifuel 0 --split_queries always"
+private let cheney_forward_normal_old_target_preserved
+  (minor: minor_state) (cs: cheney_state) (addr: U64.t) (x: U64.t)
+  : Lemma
+    (requires inj_inv cs /\
+              fwd_classified cs /\
+              well_formed_heap_part4 cs.cs_major /\
+              well_formed_heap_part1 cs.cs_major /\
+              AllocLemmas.fl_valid cs.cs_major cs.cs_fp (heap_size / U64.v mword) /\
+              AllocLemmas.fl_chain_terminates cs.cs_major cs.cs_fp (heap_size / U64.v mword) /\
+              chain_objects_blue cs.cs_major cs.cs_fp /\
+              Seq.mem addr (minor_objects minor) /\
+               cs.cs_fwd addr = 0UL /\
+               minor_wosize minor addr > 0 /\
+               (promote_object minor cs.cs_major addr cs.cs_fp (minor_wosize minor addr)).new_addr <> 0UL /\
+               x <> addr /\
+               is_val_addr (cs.cs_fwd x) /\
+               (cheney_forward_normal minor cs addr).cs_fwd x <> 0UL /\
+               is_val_addr ((cheney_forward_normal minor cs addr).cs_fwd x) /\
+               is_infix ((cheney_forward_normal minor cs addr).cs_fwd x) (cheney_forward_normal minor cs addr).cs_major = false)
+    (ensures
+      (let cs' = cheney_forward_normal minor cs addr in
+       let t : obj_addr = cs.cs_fwd x in
+       Seq.mem t (objects zero_addr cs.cs_major) /\
+       is_infix t cs.cs_major = false /\
+       is_blue t cs.cs_major = false /\
+       Seq.mem t (objects zero_addr cs'.cs_major) /\
+       is_blue t cs'.cs_major = false))
+  =
+  let wz = minor_wosize minor addr in
+  let cs' = cheney_forward_normal minor cs addr in
+  let res = promote_object minor cs.cs_major addr cs.cs_fp wz in
+  cheney_forward_normal_success minor cs addr;
+  cheney_forward_normal_other_fwd minor cs addr x;
+  promote_object_success minor cs.cs_major addr cs.cs_fp wz;
+  assert (cs'.cs_fwd x == cs.cs_fwd x);
+  assert (cs'.cs_major == res.major_out);
+  assert (is_val_addr (cs.cs_fwd x));
+  let t : obj_addr = cs.cs_fwd x in
+  if Seq.mem t (objects zero_addr cs.cs_major) then begin
+    assert (~(is_infix t cs.cs_major));
+    assert (is_infix t cs.cs_major = false);
+    assert (is_blue t cs.cs_major = false);
+    promote_object_preserves_old_target_not_blue minor cs.cs_major addr cs.cs_fp wz t
+  end else begin
+    // From fwd_classified, since ~(Seq.mem t (objects ...)), we're in the infix case.
+    // We derive a contradiction: promote_preserves_is_infix_frame shows
+    // is_infix t cs'.cs_major, but the requires says is_infix t cs'.cs_major = false.
+    assert (is_infix t cs.cs_major);
+    let goal_type = (Seq.mem t (objects zero_addr cs.cs_major) /\
+                     is_infix t cs.cs_major = false /\
+                     is_blue t cs.cs_major = false /\
+                     Seq.mem t (objects zero_addr cs'.cs_major) /\
+                     is_blue t cs'.cs_major = false) in
+    let proof (p: obj_addr) : Lemma
+      (requires Seq.mem p (objects zero_addr cs.cs_major) /\
+                is_blue p cs.cs_major = false /\
+                U64.v (cs.cs_fwd x) - 8 >= U64.v p /\
+                U64.v (cs.cs_fwd x) <=
+                  U64.v p + U64.v (wosize_of_object p cs.cs_major) * 8)
+      (ensures goal_type)
+      =
+        hd_address_spec t;
+        assert (U64.v (hd_address t) == U64.v t - 8);
+        assert (U64.v (hd_address t) >= U64.v p);
+        assert (U64.v (hd_address t) + 8 == U64.v t);
+        assert (U64.v (hd_address t) + 8 <=
+          U64.v p + U64.v (wosize_of_object p cs.cs_major) * 8);
+        promote_preserves_is_infix_frame minor cs.cs_major addr cs.cs_fp wz t p;
+        // This gives is_infix t res.major_out, hence is_infix t cs'.cs_major
+        // But requires says is_infix t cs'.cs_major = false → contradiction
+        assert (is_infix t res.major_out);
+        assert (is_infix t cs'.cs_major);
+        assert (False)
+    in
+    FStar.Classical.exists_elim goal_type #obj_addr
+      #(fun p -> Seq.mem p (objects zero_addr cs.cs_major) /\
+                 is_blue p cs.cs_major = false /\
+                 U64.v (cs.cs_fwd x) - 8 >= U64.v p /\
+                 U64.v (cs.cs_fwd x) <=
+                   U64.v p + U64.v (wosize_of_object p cs.cs_major) * 8)
+      ()
+      (fun p -> FStar.Classical.move_requires proof p)
+  end
+#pop-options
+
+#push-options "--z3rlimit 300 --fuel 1 --ifuel 0 --split_queries always"
+private let cheney_forward_normal_preserves_inj_inv
+  (minor: minor_state) (cs: cheney_state) (addr: U64.t)
+  : Lemma (requires inj_inv cs /\
+                    fwd_classified cs /\
+                    well_formed_heap_part4 cs.cs_major /\
+                    well_formed_heap_part1 cs.cs_major /\
+                    AllocLemmas.fl_valid cs.cs_major cs.cs_fp (heap_size / U64.v mword) /\
+                    AllocLemmas.fl_chain_terminates cs.cs_major cs.cs_fp (heap_size / U64.v mword) /\
+                    chain_objects_blue cs.cs_major cs.cs_fp /\
+                    minor_wf minor)
+          (ensures inj_inv (cheney_forward_normal minor cs addr))
+  =
+  if not (Seq.mem addr (minor_objects minor)) || cs.cs_fwd addr <> 0UL then
+    cheney_forward_normal_noop minor cs addr
+  else
+    let wz = minor_wosize minor addr in
+    if wz = 0 then
+      cheney_forward_normal_noop_wz0 minor cs addr
+    else
+      let res = promote_object minor cs.cs_major addr cs.cs_fp wz in
+      if res.new_addr = 0UL then
+        cheney_forward_normal_noop_oom minor cs addr
+      else begin
+        let cs' = cheney_forward_normal minor cs addr in
+        cheney_forward_normal_success minor cs addr;
+        promote_object_success minor cs.cs_major addr cs.cs_fp wz;
+        promote_object_new_addr_in_objects_not_blue minor cs.cs_major addr cs.cs_fp wz;
+        let aux_targets (x: U64.t) : Lemma
+          (ensures
+            (cs'.cs_fwd x <> 0UL /\
+             is_val_addr (cs'.cs_fwd x) /\
+             is_infix (cs'.cs_fwd x) cs'.cs_major = false ==>
+             Seq.mem ((cs'.cs_fwd x) <: obj_addr) (objects zero_addr cs'.cs_major) /\
+             is_blue ((cs'.cs_fwd x) <: obj_addr) cs'.cs_major = false)) =
+          FStar.Classical.impl_intro_gen
+            #(cs'.cs_fwd x <> 0UL /\
+              is_val_addr (cs'.cs_fwd x) /\
+              is_infix (cs'.cs_fwd x) cs'.cs_major = false)
+            #(fun (_: squash (cs'.cs_fwd x <> 0UL /\
+                              is_val_addr (cs'.cs_fwd x) /\
+                              is_infix (cs'.cs_fwd x) cs'.cs_major = false)) ->
+              Seq.mem ((cs'.cs_fwd x) <: obj_addr) (objects zero_addr cs'.cs_major) /\
+              is_blue ((cs'.cs_fwd x) <: obj_addr) cs'.cs_major = false)
+            (fun _ ->
+              assert (cs'.cs_fwd x <> 0UL);
+              assert (is_val_addr (cs'.cs_fwd x));
+              assert (is_infix (cs'.cs_fwd x) cs'.cs_major = false);
+              if x = addr then begin
+                assert (cs'.cs_fwd addr == res.new_addr);
+                assert (Seq.mem (res.new_addr <: obj_addr) (objects zero_addr res.major_out));
+                assert (is_blue (res.new_addr <: obj_addr) res.major_out = false)
+              end else begin
+                cheney_forward_normal_other_fwd minor cs addr x;
+                assert (cs'.cs_fwd x == cs.cs_fwd x);
+                assert (is_val_addr (cs.cs_fwd x));
+                cheney_forward_normal_old_target_preserved minor cs addr x
+              end)
+        in
+        FStar.Classical.forall_intro aux_targets;
+        let aux_inj (x y: U64.t) : Lemma
+          (requires cs'.cs_fwd x <> 0UL /\ cs'.cs_fwd y <> 0UL /\
+                    is_val_addr (cs'.cs_fwd x) /\ is_val_addr (cs'.cs_fwd y) /\
+                    is_infix (cs'.cs_fwd x) cs'.cs_major = false /\
+                    is_infix (cs'.cs_fwd y) cs'.cs_major = false /\
+                    cs'.cs_fwd x = cs'.cs_fwd y)
+          (ensures x = y) =
+          if x = addr then begin
+            if y = addr then ()
+            else begin
+              cheney_forward_normal_other_fwd minor cs addr y;
+              assert (cs'.cs_fwd y == cs.cs_fwd y);
+              assert (is_val_addr (cs.cs_fwd y));
+              cheney_forward_normal_old_target_preserved minor cs addr y;
+              let ty : obj_addr = cs.cs_fwd y in
+              chain_avoids_from_blue cs.cs_major cs.cs_fp ty;
+              AllocProps.alloc_spec_obj_ne_excl cs.cs_major cs.cs_fp wz ty;
+              assert (res.new_addr <> ty);
+              assert (cs'.cs_fwd addr == res.new_addr);
+              assert (res.new_addr == ty)
+            end
+          end else if y = addr then begin
+            cheney_forward_normal_other_fwd minor cs addr x;
+            assert (cs'.cs_fwd x == cs.cs_fwd x);
+            assert (is_val_addr (cs.cs_fwd x));
+            cheney_forward_normal_old_target_preserved minor cs addr x;
+            let tx : obj_addr = cs.cs_fwd x in
+            chain_avoids_from_blue cs.cs_major cs.cs_fp tx;
+            AllocProps.alloc_spec_obj_ne_excl cs.cs_major cs.cs_fp wz tx;
+            assert (res.new_addr <> tx);
+            assert (cs'.cs_fwd addr == res.new_addr);
+            assert (res.new_addr == tx)
+          end else begin
+            cheney_forward_normal_other_fwd minor cs addr x;
+            cheney_forward_normal_other_fwd minor cs addr y;
+            assert (cs'.cs_fwd x == cs.cs_fwd x);
+            assert (cs'.cs_fwd y == cs.cs_fwd y);
+            assert (is_val_addr (cs.cs_fwd x));
+            assert (is_val_addr (cs.cs_fwd y));
+            cheney_forward_normal_old_target_preserved minor cs addr x;
+            cheney_forward_normal_old_target_preserved minor cs addr y;
+            assert (cs.cs_fwd x <> 0UL);
+            assert (cs.cs_fwd y <> 0UL);
+            assert (is_val_addr (cs.cs_fwd x));
+            assert (is_val_addr (cs.cs_fwd y));
+            assert (is_infix (cs.cs_fwd x) cs.cs_major = false);
+            assert (is_infix (cs.cs_fwd y) cs.cs_major = false);
+            assert (cs.cs_fwd x = cs.cs_fwd y);
+            assert (x = y)
+          end
+        in
+        FStar.Classical.forall_intro_2 (FStar.Classical.move_requires_2 aux_inj)
+      end
+#pop-options
+
+#push-options "--z3rlimit 300 --fuel 1 --ifuel 0 --split_queries always"
+private let cheney_forward_one_preserves_inj_inv
+  (minor: minor_state) (cs: cheney_state) (addr: U64.t)
+  : Lemma (requires inj_inv cs /\
+                    fwd_classified cs /\
+                    infix_fwd_ready minor cs /\
+                    well_formed_heap_part4 cs.cs_major /\
+                    well_formed_heap_part1 cs.cs_major /\
+                    AllocLemmas.fl_valid cs.cs_major cs.cs_fp (heap_size / U64.v mword) /\
+                    AllocLemmas.fl_chain_terminates cs.cs_major cs.cs_fp (heap_size / U64.v mword) /\
+                    chain_objects_blue cs.cs_major cs.cs_fp /\
+                    minor_infix_wf minor /\
+                    minor_wf minor)
+          (ensures inj_inv (cheney_forward_one minor cs addr))
+  =
+  if cs.cs_fwd addr <> 0UL then
+    cheney_forward_one_noop minor cs addr
+  else if is_infix_in_minor minor addr then begin
+    reveal_opaque (`%minor_infix_wf) (minor_infix_wf minor);
+    cheney_forward_one_infix minor cs addr;
+    let parent = infix_parent minor addr in
+    cheney_forward_normal_preserves_inj_inv minor cs parent;
+    cheney_forward_normal_preserves_fwd_classified minor cs parent;
+    cheney_forward_normal_preserves_infix_fwd_ready minor cs parent;
+    cheney_forward_normal_preserves_wfh_part4_local minor cs parent;
+    cheney_forward_normal_preserves_wfh_part1 minor cs parent;
+    cheney_forward_normal_preserves_cob minor cs parent;
+    let cs' = cheney_forward_normal minor cs parent in
+    if not (cs'.cs_fwd parent <> 0UL &&
+            U64.v addr >= U64.v parent &&
+            U64.v (cs'.cs_fwd parent) + (U64.v addr - U64.v parent) < heap_size) then begin
+      cheney_forward_one_infix_guard_fail minor cs addr;
+      assert (cheney_forward_one minor cs addr == cs')
+    end else begin
+      cheney_forward_one_infix_guard_pass minor cs addr;
+      let delta = U64.v addr - U64.v parent in
+      let sum = U64.uint_to_t (U64.v (cs'.cs_fwd parent) + delta) in
+      let r = cheney_forward_one minor cs addr in
+      assert (r.cs_fwd == extend_forwarding cs'.cs_fwd addr sum);
+      assert (r.cs_major == cs'.cs_major);
+      let aux_targets (x: U64.t) : Lemma
+        (ensures
+          (r.cs_fwd x <> 0UL /\
+           is_val_addr (r.cs_fwd x) /\
+           is_infix (r.cs_fwd x) r.cs_major = false ==>
+           Seq.mem ((r.cs_fwd x) <: obj_addr) (objects zero_addr r.cs_major) /\
+           is_blue ((r.cs_fwd x) <: obj_addr) r.cs_major = false)) =
+        FStar.Classical.impl_intro_gen
+          #(r.cs_fwd x <> 0UL /\
+            is_val_addr (r.cs_fwd x) /\
+            is_infix (r.cs_fwd x) r.cs_major = false)
+          #(fun (_: squash (r.cs_fwd x <> 0UL /\
+                            is_val_addr (r.cs_fwd x) /\
+                            is_infix (r.cs_fwd x) r.cs_major = false)) ->
+            Seq.mem ((r.cs_fwd x) <: obj_addr) (objects zero_addr r.cs_major) /\
+            is_blue ((r.cs_fwd x) <: obj_addr) r.cs_major = false)
+          (fun _ ->
+            assert (r.cs_fwd x <> 0UL);
+            assert (is_val_addr (r.cs_fwd x));
+            assert (is_infix (r.cs_fwd x) r.cs_major = false);
+            if x = addr then begin
+              assert (r.cs_fwd addr == sum);
+              infix_parent_value minor addr;
+              let wz_infix = minor_wosize minor addr in
+              assert (delta == wz_infix * 8);
+              reveal_opaque (`%minor_infix_wf) (minor_infix_wf minor);
+              assert (wz_infix > 0);
+              FStar.Math.Lemmas.multiple_modulo_lemma wz_infix 8;
+              assert (delta % U64.v mword == 0);
+              assert (U64.v (r.cs_fwd addr) == U64.v (cs'.cs_fwd parent) + delta);
+              assert (U64.v (r.cs_fwd addr) % U64.v mword == 0);
+              assert (U64.v (cs'.cs_fwd parent) == U64.v (r.cs_fwd addr) - delta);
+              FStar.Math.Lemmas.lemma_mod_sub_distr (U64.v (r.cs_fwd addr)) delta (U64.v mword);
+              assert (U64.v (cs'.cs_fwd parent) % U64.v mword == 0);
+              assert (cs'.cs_fwd parent <> 0UL);
+              assert (U64.v (cs'.cs_fwd parent) >= U64.v mword);
+              assert (is_infix sum cs'.cs_major);
+              assert (is_infix (r.cs_fwd addr) r.cs_major);
+              assert (is_infix (r.cs_fwd addr) r.cs_major = false)
+            end else begin
+              cheney_forward_one_infix_fwd minor cs addr x;
+              assert (r.cs_fwd x == cs'.cs_fwd x)
+            end)
+      in
+      FStar.Classical.forall_intro aux_targets;
+      let aux_inj (x y: U64.t) : Lemma
+        (requires r.cs_fwd x <> 0UL /\ r.cs_fwd y <> 0UL /\
+                  is_val_addr (r.cs_fwd x) /\ is_val_addr (r.cs_fwd y) /\
+                  is_infix (r.cs_fwd x) r.cs_major = false /\
+                  is_infix (r.cs_fwd y) r.cs_major = false /\
+                  r.cs_fwd x = r.cs_fwd y)
+        (ensures x = y) =
+        if x = addr then begin
+          assert (r.cs_fwd addr == sum);
+          infix_parent_value minor addr;
+          let wz_infix = minor_wosize minor addr in
+          assert (delta == wz_infix * 8);
+          reveal_opaque (`%minor_infix_wf) (minor_infix_wf minor);
+          assert (wz_infix > 0);
+          FStar.Math.Lemmas.multiple_modulo_lemma wz_infix 8;
+          assert (delta % U64.v mword == 0);
+          assert (U64.v (r.cs_fwd addr) == U64.v (cs'.cs_fwd parent) + delta);
+          assert (U64.v (r.cs_fwd addr) % U64.v mword == 0);
+          assert (U64.v (cs'.cs_fwd parent) == U64.v (r.cs_fwd addr) - delta);
+          FStar.Math.Lemmas.lemma_mod_sub_distr (U64.v (r.cs_fwd addr)) delta (U64.v mword);
+          assert (U64.v (cs'.cs_fwd parent) % U64.v mword == 0);
+          assert (cs'.cs_fwd parent <> 0UL);
+          assert (U64.v (cs'.cs_fwd parent) >= U64.v mword);
+          assert (is_infix sum cs'.cs_major);
+          assert (is_infix (r.cs_fwd addr) r.cs_major);
+          assert (is_infix (r.cs_fwd addr) r.cs_major = false)
+        end else if y = addr then begin
+          assert (r.cs_fwd addr == sum);
+          infix_parent_value minor addr;
+          let wz_infix = minor_wosize minor addr in
+          assert (delta == wz_infix * 8);
+          reveal_opaque (`%minor_infix_wf) (minor_infix_wf minor);
+          assert (wz_infix > 0);
+          FStar.Math.Lemmas.multiple_modulo_lemma wz_infix 8;
+          assert (delta % U64.v mword == 0);
+          assert (U64.v (r.cs_fwd addr) == U64.v (cs'.cs_fwd parent) + delta);
+          assert (U64.v (r.cs_fwd addr) % U64.v mword == 0);
+          assert (U64.v (cs'.cs_fwd parent) == U64.v (r.cs_fwd addr) - delta);
+          FStar.Math.Lemmas.lemma_mod_sub_distr (U64.v (r.cs_fwd addr)) delta (U64.v mword);
+          assert (U64.v (cs'.cs_fwd parent) % U64.v mword == 0);
+          assert (cs'.cs_fwd parent <> 0UL);
+          assert (U64.v (cs'.cs_fwd parent) >= U64.v mword);
+          assert (is_infix sum cs'.cs_major);
+          assert (is_infix (r.cs_fwd addr) r.cs_major);
+          assert (is_infix (r.cs_fwd addr) r.cs_major = false)
+        end else begin
+          cheney_forward_one_infix_fwd minor cs addr x;
+          cheney_forward_one_infix_fwd minor cs addr y;
+          assert (r.cs_fwd x == cs'.cs_fwd x);
+          assert (r.cs_fwd y == cs'.cs_fwd y);
+          assert (x = y)
+        end
+      in
+      FStar.Classical.forall_intro_2 (FStar.Classical.move_requires_2 aux_inj)
+    end
+  end else begin
+    cheney_forward_one_normal minor cs addr;
+    cheney_forward_normal_preserves_inj_inv minor cs addr
+  end
+#pop-options
+
+#push-options "--z3rlimit 120 --fuel 1 --ifuel 0 --split_queries always"
+private let rec cheney_forward_fields_preserves_inj_inv
+  (minor: minor_state) (cs: cheney_state) (parent: U64.t) (i: nat) (wosize: nat)
+  : Lemma (requires inj_inv cs /\
+                    fwd_classified cs /\
+                    infix_fwd_ready minor cs /\
+                    well_formed_heap_part4 cs.cs_major /\
+                    well_formed_heap_part1 cs.cs_major /\
+                    AllocLemmas.fl_valid cs.cs_major cs.cs_fp (heap_size / U64.v mword) /\
+                    AllocLemmas.fl_chain_terminates cs.cs_major cs.cs_fp (heap_size / U64.v mword) /\
+                    chain_objects_blue cs.cs_major cs.cs_fp /\
+                    minor_infix_wf minor /\
+                    minor_wf minor)
+          (ensures inj_inv (cheney_forward_fields minor cs parent i wosize))
+          (decreases (if i < wosize then wosize - i else 0))
+  =
+  if i >= wosize then
+    cheney_forward_fields_base minor cs parent i wosize
+  else begin
+    cheney_forward_fields_step minor cs parent i wosize;
+    let field_val = to_minor_offset (minor_read_field minor parent i) in
+    cheney_forward_one_preserves_inj_inv minor cs field_val;
+    cheney_forward_one_preserves_fwd_classified minor cs field_val;
+    cheney_forward_one_preserves_infix_fwd_ready minor cs field_val;
+    cheney_forward_one_preserves_wfh_part4_local minor cs field_val;
+    cheney_forward_one_preserves_wfh_part1 minor cs field_val;
+    cheney_forward_one_preserves_cob minor cs field_val;
+    let cs' = cheney_forward_one minor cs field_val in
+    cheney_forward_fields_preserves_inj_inv minor cs' parent (i + 1) wosize
+  end
+#pop-options
+
+#push-options "--z3rlimit 100 --fuel 1 --ifuel 0 --split_queries always"
+private let rec cheney_forward_roots_preserves_inj_inv
+  (minor: minor_state) (cs: cheney_state) (roots: seq U64.t) (ridx: nat)
+  : Lemma (requires inj_inv cs /\
+                    fwd_classified cs /\
+                    infix_fwd_ready minor cs /\
+                    well_formed_heap_part4 cs.cs_major /\
+                    well_formed_heap_part1 cs.cs_major /\
+                    AllocLemmas.fl_valid cs.cs_major cs.cs_fp (heap_size / U64.v mword) /\
+                    AllocLemmas.fl_chain_terminates cs.cs_major cs.cs_fp (heap_size / U64.v mword) /\
+                    chain_objects_blue cs.cs_major cs.cs_fp /\
+                    minor_infix_wf minor /\
+                    minor_wf minor)
+          (ensures inj_inv (cheney_forward_roots minor cs roots ridx))
+          (decreases (if ridx < Seq.length roots then Seq.length roots - ridx else 0))
+  =
+  if ridx >= Seq.length roots then
+    cheney_forward_roots_base minor cs roots ridx
+  else begin
+    cheney_forward_roots_step minor cs roots ridx;
+    let r = Seq.index roots ridx in
+    cheney_forward_one_preserves_inj_inv minor cs r;
+    cheney_forward_one_preserves_fwd_classified minor cs r;
+    cheney_forward_one_preserves_infix_fwd_ready minor cs r;
+    cheney_forward_one_preserves_wfh_part4_local minor cs r;
+    cheney_forward_one_preserves_wfh_part1 minor cs r;
+    cheney_forward_one_preserves_cob minor cs r;
+    let cs' = cheney_forward_one minor cs r in
+    cheney_forward_roots_preserves_inj_inv minor cs' roots (ridx + 1)
+  end
+#pop-options
+
+#push-options "--z3rlimit 180 --fuel 1 --ifuel 0 --split_queries always"
+private let rec cheney_scan_preserves_inj_inv
+  (minor: minor_state) (cs: cheney_state) (scan: nat) (fuel: nat)
+  : Lemma (requires inj_inv cs /\
+                    fwd_classified cs /\
+                    infix_fwd_ready minor cs /\
+                    well_formed_heap_part4 cs.cs_major /\
+                    well_formed_heap_part1 cs.cs_major /\
+                    AllocLemmas.fl_valid cs.cs_major cs.cs_fp (heap_size / U64.v mword) /\
+                    AllocLemmas.fl_chain_terminates cs.cs_major cs.cs_fp (heap_size / U64.v mword) /\
+                    chain_objects_blue cs.cs_major cs.cs_fp /\
+                    minor_infix_wf minor /\
+                    minor_wf minor)
+          (ensures inj_inv (cheney_scan minor cs scan fuel))
+          (decreases fuel)
+  =
+  if fuel > 0 then begin
+    if scan >= Seq.length cs.cs_queue then
+      cheney_scan_base minor cs scan fuel
+    else begin
+      cheney_scan_step minor cs scan fuel;
+      let obj = Seq.index cs.cs_queue scan in
+      let wz = minor_wosize minor obj in
+      cheney_forward_fields_preserves_inj_inv minor cs obj 0 wz;
+      cheney_forward_fields_preserves_fwd_classified minor cs obj 0 wz;
+      cheney_forward_fields_preserves_wfh_part4_local minor cs obj 0 wz;
+      cheney_forward_fields_preserves_wfh_part1 minor cs obj 0 wz;
+      cheney_forward_fields_preserves_cob minor cs obj 0 wz;
+      let cs' = cheney_forward_fields minor cs obj 0 wz in
+      let fuel' : nat = fuel - 1 in
+      assert (fuel' < fuel);
+      cheney_scan_preserves_inj_inv minor cs' (scan + 1) fuel'
+    end
+  end else
+    cheney_scan_base minor cs scan fuel
+#pop-options
+
+#push-options "--z3rlimit 80 --fuel 0 --ifuel 0"
+private let cheney_promote_inj_inv
+  (minor: minor_state) (major: heap) (fp: U64.t) (roots: seq U64.t)
+  : Lemma (requires well_formed_heap major /\
+                    AllocLemmas.fl_valid major fp (heap_size / U64.v mword) /\
+                    AllocLemmas.fl_chain_terminates major fp (heap_size / U64.v mword) /\
+                    chain_objects_blue major fp /\
+                    minor_infix_wf minor /\
+                    minor_wf minor)
+          (ensures inj_inv
+                     ({ cs_major = (cheney_promote minor major fp roots).major_final;
+                        cs_fp = (cheney_promote minor major fp roots).fp_final;
+                        cs_fwd = (cheney_promote minor major fp roots).fwd_map;
+                        cs_queue = Seq.empty }))
+  =
+  reveal_opaque (`%well_formed_heap) well_formed_heap;
+  let cs0 : cheney_state =
+    { cs_major = major; cs_fp = fp;
+      cs_fwd = empty_forwarding; cs_queue = Seq.empty } in
+  assert (inj_inv cs0);
+  assert (fwd_classified cs0);
+  assert (infix_fwd_ready minor cs0);
+  cheney_forward_roots_preserves_inj_inv minor cs0 roots 0;
+  cheney_forward_roots_preserves_fwd_classified minor cs0 roots 0;
+  cheney_forward_roots_preserves_wfh_part4_local minor cs0 roots 0;
+  cheney_forward_roots_preserves_wfh_part1 minor cs0 roots 0;
+  cheney_forward_roots_preserves_cob minor cs0 roots 0;
+  let cs1 = cheney_forward_roots minor cs0 roots 0 in
+  cheney_scan_preserves_inj_inv minor cs1 0 (cheney_fuel minor)
+#pop-options
+
+#push-options "--z3rlimit 10 --fuel 0 --ifuel 0"
+let cheney_promote_fwd_normal_injective
+  (minor: minor_state) (major: heap) (fp: U64.t) (roots: seq U64.t)
+  : Lemma (requires well_formed_heap major /\
+                    AllocLemmas.fl_valid major fp (heap_size / U64.v mword) /\
+                    AllocLemmas.fl_chain_terminates major fp (heap_size / U64.v mword) /\
+                    chain_objects_blue major fp /\
+                    minor_infix_wf minor /\
+                    minor_wf minor)
+          (ensures fwd_normal_injective (cheney_promote minor major fp roots).fwd_map
+                                         (cheney_promote minor major fp roots).major_final)
+  = cheney_promote_inj_inv minor major fp roots
+
+let cheney_promote_fwd_targets_not_blue
+  (minor: minor_state) (major: heap) (fp: U64.t) (roots: seq U64.t)
+  : Lemma (requires well_formed_heap major /\
+                    AllocLemmas.fl_valid major fp (heap_size / U64.v mword) /\
+                    AllocLemmas.fl_chain_terminates major fp (heap_size / U64.v mword) /\
+                    chain_objects_blue major fp /\
+                    minor_infix_wf minor /\
+                    minor_wf minor)
+          (ensures fwd_targets_not_blue (cheney_promote minor major fp roots).fwd_map
+                                        (cheney_promote minor major fp roots).major_final)
+  = cheney_promote_inj_inv minor major fp roots
+#pop-options
