generational/spec/GC.Gen.CheneyPreservation.Injectivity.fsti
@@ -1,0 +1,53 @@
+/// ---------------------------------------------------------------------------
+/// GC.Gen.CheneyPreservation.Injectivity -- forwarding injectivity interface
+/// ---------------------------------------------------------------------------
+
+module GC.Gen.CheneyPreservation.Injectivity
+
+open FStar.Seq
+module U64 = FStar.UInt64
+
+open GC.Spec.Base
+open GC.Spec.Heap
+open GC.Spec.Object
+open GC.Spec.Fields
+open GC.Gen.Base
+open GC.Gen.MinorHeap
+open GC.Gen.Promote
+open GC.Gen.Cheney
+
+module AllocLemmas = GC.Spec.Allocator.Lemmas
+
+let fwd_normal_injective (fwd: forwarding_map) (g: heap) : prop =
+  forall (x y: U64.t). fwd x <> 0UL /\ fwd y <> 0UL /\
+    is_val_addr (fwd x) /\ is_val_addr (fwd y) /\
+    is_infix (fwd x) g = false /\ is_infix (fwd y) g = false /\
+    fwd x = fwd y ==> x = y
+
+let fwd_targets_not_blue (fwd: forwarding_map) (g: heap) : prop =
+  forall (x: U64.t). fwd x <> 0UL /\ is_val_addr (fwd x) /\
+    is_infix (fwd x) g = false ==>
+    Seq.mem ((fwd x) <: obj_addr) (objects zero_addr g) /\
+    is_blue ((fwd x) <: obj_addr) g = false
+
+val cheney_promote_fwd_normal_injective
+  (minor: minor_state) (major: heap) (fp: U64.t) (roots: seq U64.t)
+  : Lemma (requires well_formed_heap major /\
+                    AllocLemmas.fl_valid major fp (heap_size / U64.v mword) /\
+                    AllocLemmas.fl_chain_terminates major fp (heap_size / U64.v mword) /\
+                    chain_objects_blue major fp /\
+                    minor_infix_wf minor /\
+                    minor_wf minor)
+           (ensures fwd_normal_injective (cheney_promote minor major fp roots).fwd_map
+                                         (cheney_promote minor major fp roots).major_final)
+
+val cheney_promote_fwd_targets_not_blue
+  (minor: minor_state) (major: heap) (fp: U64.t) (roots: seq U64.t)
+  : Lemma (requires well_formed_heap major /\
+                    AllocLemmas.fl_valid major fp (heap_size / U64.v mword) /\
+                    AllocLemmas.fl_chain_terminates major fp (heap_size / U64.v mword) /\
+                    chain_objects_blue major fp /\
+                    minor_infix_wf minor /\
+                    minor_wf minor)
+          (ensures fwd_targets_not_blue (cheney_promote minor major fp roots).fwd_map
+                                        (cheney_promote minor major fp roots).major_final)
