generational/spec/GC.Gen.CheneyPreservation.NonBlueOrigin.fsti
@@ -1,0 +1,36 @@
+/// ---------------------------------------------------------------------------
+/// GC.Gen.CheneyPreservation.NonBlueOrigin
+/// ---------------------------------------------------------------------------
+
+module GC.Gen.CheneyPreservation.NonBlueOrigin
+
+open FStar.Seq
+module U64 = FStar.UInt64
+
+open GC.Spec.Base
+open GC.Spec.Heap
+open GC.Spec.Object
+open GC.Spec.Fields
+open GC.Gen.Base
+open GC.Gen.MinorHeap
+open GC.Gen.Promote
+open GC.Gen.Cheney
+
+module AllocLemmas = GC.Spec.Allocator.Lemmas
+
+val cheney_promote_nonblue_origin
+  (minor: minor_state) (major: heap) (fp: U64.t) (roots: seq U64.t)
+  (obj: obj_addr)
+  : Lemma (requires well_formed_heap major /\
+                    AllocLemmas.fl_valid major fp (heap_size / U64.v mword) /\
+                    AllocLemmas.fl_chain_terminates major fp (heap_size / U64.v mword) /\
+                    chain_objects_blue major fp /\
+                    minor_infix_wf minor /\
+                    minor_wf minor /\
+                    (let res = cheney_promote minor major fp roots in
+                     Seq.mem obj (objects zero_addr res.major_final) /\
+                     is_blue obj res.major_final = false /\
+                     ~(Seq.mem obj (objects zero_addr major) /\
+                       is_blue obj major = false)))
+          (ensures (let res = cheney_promote minor major fp roots in
+                    exists (x: U64.t). res.fwd_map x == obj /\ is_minor_pointer x))
